theories/Decidable.v
@@ -1,16 +1,129 @@
-(** * Notation for decidable propositions *)
+(**  A small library for decidable propositions based on type classes. *)
 Require Import Arith.
+Require Import Autosubst.Basics.
 
-Definition dec (X : Prop) : Type := {X} + {~ X}.
-Class Dec (X : Prop) : Type := decide : dec X.
+(* Definition dec (X : Type) : Type := (X + (X -> False))%type. *)
+Notation dec X := (X + (X -> False))%type.
+
+Class Dec (X : Type) : Type := decide : dec X.
 Arguments decide X {_}.
 
-Ltac gen_Dec_eq := unfold Dec; unfold dec; decide equality.
-
-Instance decide_eq_nat (x y : nat) : Dec (x = y). gen_Dec_eq. Defined.
-
-Instance decide_le_nat (x y : nat) : Dec (x <= y). apply le_dec. Defined.
-
-Instance decide_lt_nat (x y : nat) : Dec (x < y). apply lt_dec. Defined.
-
 Tactic Notation "decide" constr(p) := destruct (decide p).
+
+Instance decidable_neg(P : Prop) (DecP : Dec P) : Dec (~P).
+decide P. 
++ now right.
++ now left.
+Qed.
+
+Ltac eq_dec_decend s t :=
+  first[left; congruence
+       | right; congruence
+       | match s with ?s1 ?s2 => match t with ?t1 ?t2 =>
+           decide (s2 = t2);[eq_dec_decend s1 t1 | right; congruence]
+         end end
+       | idtac].
+
+Ltac derive_Dec_eq_step := cbv; match goal with
+                                   |- ((?s = ?t) + _)%type => destruct s; destruct t;
+                                                       match goal with |- ((?s = ?t) + _)%type =>
+                                                                       eq_dec_decend s t
+                                                       end
+                               end.
+
+
+
+
+Ltac derive_Dec_eq :=
+  repeat intro; match goal with |- Dec(?s = ?t) =>
+           revert s t; let H1 := fresh "H" in fix H1 1; intros; try derive_Dec_eq_step
+      end.
+(*unfold Dec; unfold dec; decide equality; try now apply (decide _).*)
+Hint Extern 0 (Dec (_ = _)) => derive_Dec_eq : derive.
+
+
+
+Ltac derive_Dec_eq_with T :=
+  repeat intro; match goal with |- Dec(?s = ?t) =>
+                                revert s t; let H1 := fresh "H" in let H2 := fresh "H" in
+                                                                  fix H1 1 with (H2 (s t : T) {struct s} : Dec(s=t)); intros; try derive_Dec_eq_step
+      end.
+
+
+Ltac derive_Dec_eq_with2 T1 T2 :=
+  repeat intro; match goal with |- Dec(?s = ?t) =>
+                                revert s t; let H1 := fresh "H" in
+                                            let H2 := fresh "H" in
+                                            let H3 := fresh "H" in
+                                            fix H1 1 with (H2 (s t : T1) {struct s} : Dec(s=t))
+                                                          (H3 (s t : T2) {struct s} : Dec(s=t));
+                                              intros; try derive_Dec_eq_step
+                end.
+
+Instance Dec_eq_nat (x y : nat) : Dec (x = y). derive. Defined.
+
+Instance Dec_le_nat (x y : nat) : Dec (x <= y). firstorder using le_dec. Defined.
+
+Instance Dec_lt_nat (x y : nat) : Dec (x < y). firstorder using lt_dec. Defined.
+
+Instance Dec_and (P1 P2 : Prop) {Dec_P1 : Dec P1} {Dec_P2 : Dec P2} : Dec (P1 /\ P2). cbv. decide P1. decide P2; tauto. tauto. Defined.
+
+Instance Dec_or (P1 P2 : Prop) {Dec_P1 : Dec P1} {Dec_P2 : Dec P2} : Dec (P1 \/ P2). cbv. decide P1. tauto. decide P2; tauto. Defined.
+
+Instance Dec_impl (P1 P2 : Prop) {Dec_P1 : Dec P1} {Dec_P2 : Dec P2} : Dec (P1 -> P2). cbv. decide P1. decide P2; tauto. tauto. Defined.
+
+
+Class Countable (X : Type) := {
+                               enum : nat -> X;
+                               repr : X -> nat;
+                               countableProp : forall x, enum(repr x) = x
+                             }. 
+
+Class Finite (X : Type) {CountableX : Countable X} := {
+                                                       numElems : nat;
+                                                       finiteProp : forall x, repr x < numElems
+                                                     }.
+
+Arguments numElems X {_ _}.
+
+Require Import Omega.
+
+Instance Dec_fin_quant_T (P : nat -> Prop) {DecP : forall n, Dec (P n)} (m : nat) : Dec {n | n < m /\ P n}.
+cbv. induction m.
+- right. firstorder.
+- decide (P (m)).
+  + firstorder.
+  + destruct IHm.
+    * firstorder.
+    * right. intros [n' H]. decide (n' < m); firstorder.
+      now replace n' with m in * by omega.
+Defined.
+
+Instance Dec_fin_quant (P : nat -> Prop) {DecP : forall n, Dec (P n)} (m : nat) : Dec (exists n, n < m /\ P n).
+destruct (Dec_fin_quant_T P m). left; firstorder. right; firstorder. Defined.
+
+Require Import FunctionalExtensionality.
+
+
+Lemma decide_eq_fin_domain {X Y : Type} {CountableX : Countable X} {FiniteX : Finite X} {DecEqY : forall (y1 y2 : Y), Dec (y1 = y2)}  (f g : X -> Y) :
+  (f = g) + {x | f x <> g x}.
+Proof.
+  destruct (decide {n | n < numElems _ /\ f (enum n) <> g (enum n)}) as [ H | H].
++ right.
+  destruct H as [n [H1 H2]].
+  exists (enum n). intros H. auto using equal_f.
++ left. apply functional_extensionality.
+  intros x.
+  decide (f x = g x); trivial.
+  exfalso. apply H. exists (repr x).
+  split.
+  now eauto using finiteProp.
+  now rewrite countableProp.
+Defined.
+  
+Instance Dec_eq_fin_domain {X Y : Type} {CountableX : Countable X} {FiniteX : Finite X} {DecEqY : forall (y1 y2 : Y), Dec (y1 = y2)}  (f g : X -> Y) :
+  Dec (f = g).
+destruct (decide_eq_fin_domain f g) as [H | H].
++ now left.
++ right. intro. destruct H. congruence.
+Defined.
