examples/ssr/Context.v
@@ -4,11 +4,11 @@
 Require Import ssreflect ssrfun ssrbool eqtype ssrnat seq.
 Require Import AutosubstSsr.
 
-Definition get {T} `{Ids T} (Gamma : seq T) (n : var) : T :=
+Definition get {T} `{VarConstr T} (Gamma : seq T) (n : var) : T :=
   nth (ids 0) Gamma n.
 Arguments get {T _} Gamma n.
 
-Fixpoint dget {T} `{Ids T} `{Subst T} (Gamma : list T) (n : var) {struct n} : T :=
+Fixpoint dget {T} `{VarConstr T} `{Subst T} (Gamma : list T) (n : var) {struct n} : T :=
   match Gamma, n with
     | [::], _ => ids 0
     | A :: _, 0 => A.[ren (+1)]
@@ -16,6 +16,6 @@ Fixpoint dget {T} `{Ids T} `{Subst T} (Gamma : list T) (n : var) {struct n} : T 
   end.
 Arguments dget {T _ _} Gamma n.
 
-Lemma get_map {T} `{Ids T} (f : T -> T) Gamma n :
+Lemma get_map {T} `{VarConstr T} (f : T -> T) Gamma n :
   n < size Gamma -> get (map f Gamma) n = f (get Gamma n).
 Proof. exact: nth_map. Qed.
