theories/Context.v
@@ -5,130 +5,131 @@ Require Import Autosubst.Autosubst.
 
 Fixpoint atn {X} l n (x : X) :=
   match l with
-    | nil => False
-    | y :: l' => match n with
-                  | 0 => x = y
-                  | S n' => atn l' n' x
-                end
+  | nil => False
+  | y :: l' => match n with
+              | 0 => x = y
+              | S n' => atn l' n' x
+              end
   end.
 
 
 Section SubstInstance.
 
-Context {sort : Type} {term : sort -> Type}.
-Context {Vector_sort : Vector sort} {Ids_term : Ids term} {Rename_term : Rename term}
-  {Subst_term : Subst term} {SubstLemmas_term : SubstLemmas term}.
+  Context {sort : Type} {dec_eq_sort : forall a b : sort, Dec (a = b)} {Vector_sort : Vector sort}.
 
-Context {o : sort}.
+  Context  {term : sort -> Type} {VarConstr_term : VarConstr term} {Rename_term : Rename term}
+           {Subst_term : Subst term} {SubstLemmas_term : SubstLemmas term}.
 
-Inductive atnd : list (term o) -> var -> (term o) -> Prop :=
-| Atnd0 Delta A A' :
-    A' = A.[updV  (+1)] -> atnd (A :: Delta) 0 A'
-| AtndS Delta x A B B' :
-    atnd Delta x B -> B' = B.[ren(+1)] -> atnd (A :: Delta) (S x) B'.
+  Context {o : sort}.
 
-Lemma atn_mmap {f : term -> term} {Gamma x A A'} :
-  atn Gamma x A -> A' = (f A) -> atn (mmap f Gamma) x A'.
-Proof.
-  revert x.
-  induction Gamma; intros; simpl in *; trivial.
-  destruct x; subst; eauto.
-Qed.
+  Inductive atnd : list (term o) -> var -> (term o) -> Prop :=
+  | Atnd0 Delta A A' :
+      A' = A.[ren o (+1)] -> atnd (A :: Delta) 0 A'
+  | AtndS Delta x A B B' :
+      atnd Delta x B -> B' = B.[ren o (+1)] -> atnd (A :: Delta) (S x) B'.
 
-Lemma mmap_atn {f : term -> term} {Gamma x A'} :
-  atn (mmap f Gamma) x A' -> exists A, A' = (f A) /\ atn Gamma x A.
-Proof.
-  revert x. induction Gamma; intros; simpl in *.
-  - contradiction.
-  - destruct x; subst; eauto.
-Qed.
+  Lemma atn_mmap {f : term o -> term o} {Gamma x A A'} :
+    atn Gamma x A -> A' = (f A) -> atn (mmap f Gamma) x A'.
+  Proof.
+    revert x.
+    induction Gamma; intros; simpl in *; trivial.
+    destruct x; subst; eauto.
+  Qed.
 
-Lemma up_mmap_atn zeta xi Gamma1 Gamma2 A x :
-  (forall x B, atn Gamma1 x B -> atn Gamma2 (zeta x) B.[ren xi]) ->
-  atn (mmap (subst (ren (+1))) Gamma1) x A ->
-  atn (mmap (subst (ren (+1))) Gamma2) (zeta x) A.[ren (0 .: xi >>> (+1))].
-Proof.
-  intros H1 H2.
-  edestruct (mmap_atn H2) as [? [? ?]]. subst.
-  eapply atn_mmap; eauto. autosubst.
-Qed.
+  Lemma mmap_atn {f : term o -> term o} {Gamma x A'} :
+    atn (mmap f Gamma) x A' -> exists A, A' = (f A) /\ atn Gamma x A.
+  Proof.
+    revert x. induction Gamma; intros; simpl in *.
+    - contradiction.
+    - destruct x; subst; eauto.
+  Qed.
 
-Lemma up_atnd xi Delta1 Delta2 A B x:
-  (forall x C, atnd Delta1 x C -> atnd Delta2 (xi x) C.[ren xi]) ->
-  atnd (A :: Delta1) x B ->
-  atnd (A.[ren xi] :: Delta2) ((0 .: xi >>> (+1)) x) B.[ren (0 .: xi >>> (+1))].
-Proof.
-  intros H1 H2; destruct x; simpl; inv H2; econstructor; eauto; autosubst.
-Qed.
+  (* Lemma up_mmap_atn zeta xi Gamma1 Gamma2 A x : *)
+  (*   (forall x B, atn Gamma1 x B -> atn Gamma2 (zeta x) B.[ren o xi]) -> *)
+  (*   atn (mmap (subst1 (ren o (+1))) Gamma1) x A -> *)
+  (*   atn (mmap (subst1 (ren o (+1))) Gamma2) (zeta x) A.[ren o (0 .: xi >> (+1))]. *)
+  (* Proof. *)
+  (*   intros H1 H2. *)
+  (*   edestruct (mmap_atn H2) as [? [? ?]]. subst. *)
+  (*   eapply atn_mmap; eauto. autosubst. *)
+  (* Qed. *)
 
-Lemma atnd_steps x Gamma Delta A :
-  atnd Gamma x A <->
-  atnd (Delta ++ Gamma) (length Delta + x) A.[ren(+(length Delta))].
-Proof.
-  revert A x.
-  induction Delta; intros.
-  - split.
-    + autosubst.
-    + autosubst.
-  - simpl. cutrewrite (A.[ren (+S (length Delta))] =
-                       A.[ren(+length Delta)].[ren(+1)]); [idtac|autosubst].
-    split.
-      + econstructor. eapply IHDelta; eassumption. reflexivity.
-      + intros H. inv H. rewrite IHDelta. apply lift_inj in H5.
-        subst. eassumption.
-Qed.
+  (* Lemma up_atnd xi Delta1 Delta2 A B x: *)
+  (*   (forall x C, atnd Delta1 x C -> atnd Delta2 (xi x) C.[ren o xi]) -> *)
+  (*   atnd (A :: Delta1) x B -> *)
+  (*   atnd (A.[ren o xi] :: Delta2) ((0 .: xi >> (+1)) x) B.[ren o (0 .: xi >> (+1))]. *)
+  (* Proof. *)
+  (*   intros H1 H2; destruct x; simpl; inv H2; econstructor; eauto; autosubst. *)
+  (* Qed. *)
 
-Lemma atnd_steps' x Gamma Delta A :
-  atnd (Delta ++ Gamma) (x + length Delta) A ->
-  exists B, A = B.[ren(+(length Delta))] /\ atnd Gamma x B.
-Proof.
-  revert A x.
-  induction Delta; intros.
-  - exists A.
-    simpl in H.
-    rewrite Plus.plus_0_r in H. intuition autosubst.
-  - asimpl. simpl in *.
-    rewrite plusnS in *.
-    inv H.
-    edestruct IHDelta as [B' [? ?]]; eauto. exists B'. subst.
-    intuition autosubst.
-Qed.
+  (* Lemma atnd_steps x Gamma Delta A : *)
+  (*   atnd Gamma x A <-> *)
+  (*   atnd (Delta ++ Gamma) (length Delta + x) A.[ren o (+(length Delta))]. *)
+  (* Proof. *)
+  (*   revert A x. *)
+  (*   induction Delta; intros. *)
+  (*   - split. *)
+  (*     + asimpl. *)
+  (*     + autosubst. *)
+  (*   - simpl. cutrewrite (A.[ren (+S (length Delta))] = *)
+  (*                        A.[ren(+length Delta)].[ren(+1)]); [idtac|autosubst]. *)
+  (*     split. *)
+  (*     + econstructor. eapply IHDelta; eassumption. reflexivity. *)
+  (*     + intros H. inv H. rewrite IHDelta. apply lift_inj in H5. *)
+  (*       subst. eassumption. *)
+  (* Qed. *)
 
-Corollary atnd_step Delta A x B :
-  atnd Delta x A <-> atnd (B :: Delta) (S x) A.[ren(+1)].
-Proof.
-  apply atnd_steps with (Delta := B :: nil).
-Qed.
+  (* Lemma atnd_steps' x Gamma Delta A : *)
+  (*   atnd (Delta ++ Gamma) (x + length Delta) A -> *)
+  (*   exists B, A = B.[ren o (+(length Delta))] /\ atnd Gamma x B. *)
+  (* Proof. *)
+  (*   revert A x. *)
+  (*   induction Delta; intros. *)
+  (*   - exists A. *)
+  (*     simpl in H. *)
+  (*     rewrite Plus.plus_0_r in H. intuition autosubst. *)
+  (*   - asimpl. simpl in *. *)
+  (*     rewrite plusnS in *. *)
+  (*     inv H. *)
+  (*     edestruct IHDelta as [B' [? ?]]; eauto. exists B'. subst. *)
+  (*     intuition autosubst. *)
+  (* Qed. *)
 
-Lemma atnd_repl Gamma A Delta :
-  (atnd (Delta ++ A :: Gamma) (length Delta) A.[ren(+ S (length Delta))]) /\
-  (forall x B A',
-     x <> length Delta -> atnd (Delta ++ A :: Gamma) x B ->
-     atnd (Delta ++ A' :: Gamma) x B).
-Proof.
-  split.
-  - pose proof (atnd_steps 0 (A :: Gamma) Delta A.[ren(+1)]) as H. asimpl in H.
-    apply H. now constructor.
-  - intros x. revert Gamma A Delta.
-    induction x; intros Gamma A Delta H B A' H_atn.
-    + destruct Delta as [| C Delta]. { now intuition. }
-      simpl in *.
-      inv H_atn. now constructor.
-    + destruct Delta as [| C Delta]; simpl in *.
-      * inv H_atn. econstructor. eassumption. reflexivity.
-      * inv H_atn. econstructor. eapply IHx; eauto. reflexivity.
-Qed.
+  (* Corollary atnd_step Delta A x B : *)
+  (*   atnd Delta x A <-> atnd (B :: Delta) (S x) A.[ren o(+1)]. *)
+  (* Proof. *)
+  (*   apply atnd_steps with (Delta := B :: nil). *)
+  (* Qed. *)
 
-Lemma atnd_defined Delta x : (exists B, atnd Delta x B) <-> x < length Delta.
-Proof.
-  revert x. induction Delta; intuition; asimpl in *; ainv.
-  - destruct x. omega. cut(x < length Delta). omega.
-    ainv. firstorder.
-  - destruct x.
-    + eexists. now econstructor.
-    + edestruct IHDelta as [_ [? ?]]. cut(x < length Delta); eauto. omega.
-      eexists. econstructor; eauto.
-Qed.
+  (* Lemma atnd_repl Gamma A Delta : *)
+  (*   (atnd (Delta ++ A :: Gamma) (length Delta) A.[ren o (+ S (length Delta))]) /\ *)
+  (*   (forall x B A', *)
+  (*       x <> length Delta -> atnd (Delta ++ A :: Gamma) x B -> *)
+  (*       atnd (Delta ++ A' :: Gamma) x B). *)
+  (* Proof. *)
+  (*   split. *)
+  (*   - pose proof (atnd_steps 0 (A :: Gamma) Delta A.[ren o (+1)]) as H. asimpl in H. *)
+  (*     apply H. now constructor. *)
+  (*   - intros x. revert Gamma A Delta. *)
+  (*     induction x; intros Gamma A Delta H B A' H_atn. *)
+  (*     + destruct Delta as [| C Delta]. { now intuition. } *)
+  (*                              simpl in *. *)
+  (*       inv H_atn. now constructor. *)
+  (*     + destruct Delta as [| C Delta]; simpl in *. *)
+  (*       * inv H_atn. econstructor. eassumption. reflexivity. *)
+  (*       * inv H_atn. econstructor. eapply IHx; eauto. reflexivity. *)
+  (* Qed. *)
+
+  (* Lemma atnd_defined Delta x : (exists B, atnd Delta x B) <-> x < length Delta. *)
+  (* Proof. *)
+  (*   revert x. induction Delta; intuition; asimpl in *; ainv. *)
+  (*   - destruct x. omega. cut(x < length Delta). omega. *)
+  (*     ainv. firstorder. *)
+  (*   - destruct x. *)
+  (*     + eexists. now econstructor. *)
+  (*     + edestruct IHDelta as [_ [? ?]]. cut(x < length Delta); eauto. omega. *)
+  (*       eexists. econstructor; eauto. *)
+  (* Qed. *)
 
 End SubstInstance.
 
